Core/Infer/TypeSound.lean
@@ -4,469 +4,58 @@ import Core.Infer.«Type»
 import Core.Ty
 import Core.Typing
 
+import Core.Vec
+import Lilac
+open Lilac
+
 namespace Core
-
-theorem valid_data_type_sound :
-  Ty.valid_data_type G T = some () ->
-  ValidTyHeadVariable T (is_data G) := by
-intro h
-cases T <;> simp [Ty.valid_data_type, ValidTyHeadVariable, Ty.spine] at *
-case _ => assumption
-case _ a =>
-rw[Option.bind_eq_some_iff] at h; rcases h with ⟨w, h1, h⟩
-rw[Option.bind_eq_some_iff] at h1; simp at h1; simp at h
-rcases h1 with ⟨x, sp, h1⟩
-rcases h1 with ⟨e1, e2⟩
-exists x
-have lem1 : x = w.fst := by rw[<-e2]
-have lem2 : sp ++ [a] = w.snd := by rw[<-e2]
-constructor
-· exists w.snd;
-  rw[Option.bind_eq_some_iff]; simp; exists x; exists sp
-· rw[lem1]; assumption
-
-
-theorem valid_open_type_sound :
-  Ty.valid_open_type G T = some dt ->
-  ValidTyHeadVariable T (is_opent G) := by
-intro h
-cases T <;> simp [Ty.valid_open_type, ValidTyHeadVariable, Ty.spine] at *
-case _ => assumption
-case _ a =>
-rw[Option.bind_eq_some_iff] at h; rcases h with ⟨w, h1, h⟩
-rw[Option.bind_eq_some_iff] at h1; simp at h1; simp at h
-rcases h1 with ⟨x, sp, h1⟩
-rcases h1 with ⟨e1, e2⟩
-exists x
-have lem1 : x = w.fst := by rw[<-e2]
-have lem2 : sp ++ [a] = w.snd := by rw[<-e2]
-constructor
-· exists w.snd;
-  rw[Option.bind_eq_some_iff]; simp; exists x; exists sp
-· rw[lem1]; assumption
-
-
-theorem valid_inst_type_sound :
-  Term.valid_inst_type G t = some dt ->
-  ValidHeadVariable t (is_instty G) := by
-intro h
-cases t <;> simp [Term.valid_inst_type, ValidHeadVariable, Term.spine] at *
-case _ => assumption
-all_goals (
-  case _ =>
-    rw[Option.bind_eq_some_iff] at h; rcases h with ⟨w, h1, h⟩
-    exists w.fst
-    simp at h
-    constructor;
-    exists w.snd
-    assumption
-)
-
-theorem Ty.stable_type_match_sound :
-  Ty.stable_type_match Δ A R = .some () ->
-  StableTypeMatch Δ A R := by
-intro h
-induction Δ, A, R using Ty.stable_type_match.induct <;> simp [Ty.stable_type_match] at h
-case _ ih =>
-  replace ih := ih h
-  apply StableTypeMatch.all;
-  assumption
-case _ ih =>
-  replace ih := ih h;
-  apply StableTypeMatch.arrow; assumption
-case _ ih =>
-  rw[Option.bind_eq_some_iff] at h; rcases h with ⟨_, h1, h⟩
-  simp at h; cases h
-  apply StableTypeMatch.refl
-  assumption
-
-theorem Ty.prefix_type_match_sound :
-  Ty.prefix_type_match G A R = .some T ->
-  PrefixTypeMatch G A R T := by
-intro h
-induction G, A, R using Ty.prefix_type_match.induct generalizing T <;> simp [Ty.prefix_type_match] at h
-all_goals try (case _ h' => simp at h'; exfalso; apply h' h.1)
-case _ e ih =>
-  replace e := eq_of_beq e; cases e;  simp at h;
-  replace ih := ih h
-  constructor; assumption
-case _ h' ih =>
-  rcases h with ⟨e, h⟩
-  rw[Option.bind_eq_some_iff] at h; rcases h with ⟨w, h1, h⟩
-  simp at h; rcases h with ⟨h2, h3⟩; subst e
-  replace ih := ih h1
-  have lem : w[-1][+1] = T[+1] := by rw[<-h2]; rw[<-h3]; simp
-  apply PrefixTypeMatch.all;
-  simp at lem; rw[h2] at lem; subst lem
-  assumption
-case _ h =>
-  rw[Option.bind_eq_some_iff] at h; rcases h with ⟨w, h1, h⟩
-  cases h; apply PrefixTypeMatch.refl; assumption
-
 
 theorem infer_type_sound :
   ⊢ G ->
   t.infer_type G Δ Γ = some T ->
   G&Δ, Γ ⊢ t : T := by
 intro wf h
-induction Δ, Γ, t using Term.infer_type.induct generalizing T <;> simp [Term.infer_type] at h
-all_goals try (
-  case _ =>
-  rw[Option.bind_eq_some_iff] at h; rcases h with ⟨_, h1, h⟩
-  rw[Option.bind_eq_some_iff] at h; rcases h with ⟨_, h2, h⟩
-  rw[Option.bind_eq_some_iff] at h; rcases h with ⟨_, h3, h⟩
+fun_induction Term.infer_type generalizing T <;> simp at *
+case _ => -- var
+  rw[Option.bind_eq_some_iff] at h; rcases h with ⟨h1, h2, h⟩
+  rw[Option.bind_eq_some_iff] at h; rcases h with ⟨h3, h4, h⟩
+  rw[Option.bind_eq_some_iff] at h; rcases h with ⟨h5, h6, h⟩
   cases h
-  replace h2 := infer_kind_sound h2 wf
-  replace h3 := Kind.base_kind_sound h3; subst h3
-  constructor; assumption; assumption )
-case _ ih1 ih2 ih3 ih4 => -- match
-  rw[Option.bind_eq_some_iff] at h; rcases h with ⟨_, h1, h⟩
-  rw[Option.bind_eq_some_iff] at h; rcases h with ⟨_, h2, h⟩
-  rw[Option.bind_eq_some_iff] at h; rcases h with ⟨pat_sp, h3, h⟩
-  simp at h; rcases h with ⟨h4, h⟩
-  rw[Option.bind_eq_some_iff] at h; rcases h with ⟨_, h5, h⟩
-  rw[Option.bind_eq_some_iff] at h; rcases h with ⟨_, h6, h⟩
-  rw[Option.bind_eq_some_iff] at h; rcases h with ⟨_, h8, h⟩
-  rw[Option.bind_eq_some_iff] at h; rcases h with ⟨_, h9, h⟩
-  rw[Option.bind_eq_some_iff] at h; rcases h with ⟨_, h10, h⟩
-  rw[Option.bind_eq_some_iff] at h; rcases h with ⟨_, h11, h⟩
-  simp at h; cases h.1; cases h.2; clear h
-  replace h4 := Vec.elems_eq_to_sound h4
-  replace h3 := Vec.seq_sound h3
-  replace h5 := Vec.seq_sound h5
-  replace h6 := Vec.seq_sound h6
-  replace h8 := Vec.seq_sound h8
-  replace h9 := Vec.seq_sound h9
-  replace h10 := Vec.get_elem_if_eq_sound h10;
-  apply Typing.mtch
-  apply ih1 h1
-  apply valid_data_type_sound h2
-  apply ih4 h11
-  · intro i; replace h4 := h4 i; replace h3 := h3 i
-    simp [ValidHeadVariable]; exists (pat_sp i).1;
-    constructor
-    exists (pat_sp i).2
-    assumption
-  · intro i; replace h6 := h6 i; apply ih3 i h6
-  · intro i; replace h8 := h8 i; apply Ty.stable_type_match_sound h8
-  · intro i; replace h5 := h5 i; apply ih2 i h5
-  · intro i; replace h9 := h9 i; rw[h10 i] at h9; apply Ty.prefix_type_match_sound h9
+  replace h6 := Kind.base_kind_sound h3 h6; subst h3
+  apply Typing.var
+  · apply h2
+  · apply infer_kind_sound h4
 
-case _ Δ _ _ _ _ ih1 ih2 ih3 => -- guard
-  rw[Option.bind_eq_some_iff] at h; rcases h with ⟨_, h1, h⟩
-  rw[Option.bind_eq_some_iff] at h; rcases h with ⟨_, h2, h⟩
-  rw[Option.bind_eq_some_iff] at h; rcases h with ⟨_, h3, h⟩
-  rw[Option.bind_eq_some_iff] at h; rcases h with ⟨_, h4, h⟩
-  rw[Option.bind_eq_some_iff] at h; rcases h with ⟨_, h5, h⟩
-  rw[Option.bind_eq_some_iff] at h; rcases h with ⟨_, h6, h⟩
-  rw[Option.bind_eq_some_iff] at h; rcases h with ⟨_, h8, h⟩
-  rw[Option.bind_eq_some_iff] at h; rcases h with ⟨_, h9, h⟩
-  rw[Option.bind_eq_some_iff] at h; rcases h with ⟨_, h10, h⟩
-  rw[Option.bind_eq_some_iff] at h; rcases h with ⟨_, h11, h⟩
-  rw[Option.bind_eq_some_iff] at h; rcases h with ⟨_, h12, h⟩
-  cases h
-  replace ih1 := ih1 h1; clear h1
-  replace ih2 := ih2 h2; clear h2
-  replace ih3 := ih3 h9; clear h9
-  replace h3 := infer_kind_sound h3
-  replace h4 := Kind.is_open_kind_sound h4
-  replace h5 := Ty.stable_type_match_sound (Δ := Δ) h5
-  replace h6 := valid_open_type_sound h6
-  replace h8 := valid_inst_type_sound h8
-  replace h10 := Ty.prefix_type_match_sound h10
-  apply Typing.guard
-  assumption
-  assumption
-  assumption
-  assumption
-  assumption
-  assumption
-  assumption
+case _ => -- defn
+  rw[Option.bind_eq_some_iff] at h; rcases h with ⟨h1, h2, h⟩
+  rw[Option.bind_eq_some_iff] at h; rcases h with ⟨h3, h4, h⟩; simp at h;
+  rcases h with ⟨h5, h6⟩; subst h3; subst T
+  replace h4 := infer_kind_sound h4
+  apply Typing.defn
+  apply h2
+  apply h4
 
-case _ ih => -- lam
-  rw[Option.bind_eq_some_iff] at h; rcases h with ⟨_, h1, h⟩
-  rw[Option.bind_eq_some_iff] at h; rcases h with ⟨_, h2, h⟩
-  rw[Option.bind_eq_some_iff] at h; rcases h with ⟨_, h3, h⟩
-  rw[Option.bind_eq_some_iff] at h; rcases h with ⟨_, h4, h⟩
-  rw[Option.bind_eq_some_iff] at h; rcases h with ⟨_, h5, h⟩
-  cases h
-  replace h1 := infer_kind_sound h1 wf
-  replace h2 := base_kind_some h2; cases h2
-  replace ih := ih h3
-  replace h5 := base_kind_some h5; cases h5
-  apply Typing.lam; assumption; assumption
-case _ ih1 ih2 =>
-  rw[Option.bind_eq_some_iff] at h; rcases h with ⟨_, h1, h⟩
-  rw[Option.bind_eq_some_iff] at h; rcases h with ⟨_, h2, h⟩
-  rw[Option.bind_eq_some_iff] at h; rcases h with ⟨_, h3, h⟩
-  rw[Option.bind_eq_some_iff] at h; rcases h with ⟨_, h4, h⟩
-  rw[Option.bind_eq_some_iff] at h; rcases h with ⟨_, h5, h⟩
-  simp at h; rcases h with ⟨h6, h⟩; rcases h6 with ⟨h6, h7⟩
-  subst h; subst h6; subst h7
-  replace ih1 := ih1 h1; clear h1
-  replace ih2 := ih2 h3; clear h3
-  replace h2 := Ty.is_arrow_some_sound h2
-  replace h4 := infer_kind_sound h4 wf
-  replace h5 := base_kind_some h5
-  subst h2; subst h5
-  apply Typing.app
-  assumption
-  assumption
-  assumption
+case _ ih => -- spctor
+  rw[Option.bind_eq_some_iff] at h; rcases h with ⟨h1, h2, h⟩
+  rw[Option.bind_eq_some_iff] at h; rcases h with ⟨h3, h4, h⟩; simp at h
+  rcases h with ⟨h5, h⟩
+  rw[Option.bind_eq_some_iff] at h; rcases h with ⟨h6, h7, h⟩; simp at h
+  rcases h with ⟨h8, h⟩
+  rcases h8 with ⟨h9, h10⟩
+  rcases h9 with ⟨h11, h12⟩
+  replace h4 := Vec.seq_sound h4
+  sorry
+sorry
+sorry
+sorry
+sorry
+sorry
+sorry
+sorry
+sorry
+sorry
+sorry
+sorry
+sorry
 
-case _ ih =>
-  rw[Option.bind_eq_some_iff] at h; rcases h with ⟨_, h1, h⟩
-  rw[Option.bind_eq_some_iff] at h; rcases h with ⟨_, h2, h⟩
-  rw[Option.bind_eq_some_iff] at h; rcases h with ⟨_, h3, h⟩
-  simp at h; cases h.1; cases h.2; clear h
-  rw[Option.bind_eq_some_iff] at h2; rcases h2 with ⟨_, h4, h2⟩
-  replace ih := ih h1; clear h1
-  simp at h2; cases h2.1; cases h2.1; clear h2
-  replace h3 := Kind.base_kind_sound h3; cases h3
-  replace h4 := infer_kind_sound h4 wf
-  apply Typing.lamt
-  apply Kinding.all; assumption
-  assumption
-
-case _ ih1 =>
-  rw[Option.bind_eq_some_iff] at h; rcases h with ⟨_, h1, h⟩
-  rw[Option.bind_eq_some_iff] at h; rcases h with ⟨_, h2, h⟩
-  rw[Option.bind_eq_some_iff] at h; rcases h with ⟨_, h3, h⟩
-  simp at h; cases h.1; cases h.2
-  replace ih1 := ih1 h2; clear h2
-  replace h1 := infer_kind_sound h1 wf
-  replace h3 := Ty.is_all_some_sound h3
-  subst h3
-  apply Typing.appt
-  assumption
-  assumption
-  rfl
-
-case _ ih1 ih2 =>
-  rw[Option.bind_eq_some_iff] at h; rcases h with ⟨_, h1, h⟩
-  rw[Option.bind_eq_some_iff] at h; rcases h with ⟨_, h2, h⟩
-  rw[Option.bind_eq_some_iff] at h; rcases h with ⟨_, h3, h⟩
-  rw[Option.bind_eq_some_iff] at h; rcases h with ⟨_, h4, h⟩
-  simp at h; cases h.1.1; cases h.1.2; cases h.2; clear h
-  replace ih1 := ih1 h1
-  replace ih2 := ih2 h2
-  replace h3 := infer_kind_sound h3
-  replace h4 := Ty.is_eq_some_sound h4
-  subst h4
-  apply Typing.cast
-  assumption
-  assumption
-
-case _ =>
-  rw[Option.bind_eq_some_iff] at h; rcases h with ⟨_, h1, h⟩
-  cases h
-  replace h1 := infer_kind_sound h1 wf
-  apply Typing.refl
-  assumption
-
-case _ ih =>
-  rw[Option.bind_eq_some_iff] at h; rcases h with ⟨_, h1, h⟩
-  rw[Option.bind_eq_some_iff] at h; rcases h with ⟨_, h2, h⟩
-  rw[Option.bind_eq_some_iff] at h; rcases h with ⟨_, h3, h⟩
-  cases h
-  replace ih := ih h1
-  replace h2 := infer_kind_sound h2
-  replace h3 := Ty.is_eq_some_sound h3
-  subst h3
-  apply Typing.sym
-  assumption
-
-case _ ih1 ih2 =>
-  rw[Option.bind_eq_some_iff] at h; rcases h with ⟨_, h1, h⟩
-  rw[Option.bind_eq_some_iff] at h; rcases h with ⟨_, h2, h⟩
-  rw[Option.bind_eq_some_iff] at h; rcases h with ⟨_, h3, h⟩
-  rw[Option.bind_eq_some_iff] at h; rcases h with ⟨_, h4, h⟩
-  rw[Option.bind_eq_some_iff] at h; rcases h with ⟨_, h5, h⟩
-  rw[Option.bind_eq_some_iff] at h; rcases h with ⟨_, h6, h⟩
-  simp at h; rcases h with ⟨h, e2⟩; subst e2
-  rcases h with ⟨e1, e2⟩
-  replace ih1 := ih1 h1; clear h1
-  replace ih2 := ih2 h4; clear h4
-  replace h2 := infer_kind_sound h2 wf
-  replace h3 := Ty.is_eq_some_sound h3
-  replace h5 := infer_kind_sound h5 wf
-  replace h6 := Ty.is_eq_some_sound h6
-  subst h3; subst h6
-  rw[<-e1] at h5; rw[<-e1] at ih2
-  rw[e2] at ih1; rw[e2] at h2
-  apply Typing.seq
-  assumption
-  assumption
-case _ ih1 ih2 =>
-  rw[Option.bind_eq_some_iff] at h; rcases h with ⟨_, h1, h⟩
-  rw[Option.bind_eq_some_iff] at h; rcases h with ⟨_, h2, h⟩
-  rw[Option.bind_eq_some_iff] at h; rcases h with ⟨_, h3, h⟩
-  rw[Option.bind_eq_some_iff] at h; rcases h with ⟨_, h4, h⟩
-  rw[Option.bind_eq_some_iff] at h; rcases h with ⟨_, h5, h⟩
-  rw[Option.bind_eq_some_iff] at h; rcases h with ⟨_, h6, h⟩
-  rw[Option.bind_eq_some_iff] at h; rcases h with ⟨_, h7, h⟩
-  simp at h; rcases h with ⟨e1, e2⟩; subst e2
-  replace ih1 := ih1 h1; clear h1
-  replace ih2 := ih2 h4; clear h4
-  replace h2 := infer_kind_sound h2 wf
-  replace h3 := Ty.is_eq_some_sound h3
-  replace h5 := infer_kind_sound h5 wf
-  replace h6 := Ty.is_eq_some_sound h6
-  replace h7 := Kind.is_arrow_sound h7
-  subst h3; subst h6
-  rw[<-e1] at h7; rw[h7] at ih1; rw[h7] at h2
-  apply Typing.appc
-  assumption
-  assumption
-
-case _ ih1 ih2 =>
-  rw[Option.bind_eq_some_iff] at h; rcases h with ⟨_, h1, h⟩
-  rw[Option.bind_eq_some_iff] at h; rcases h with ⟨_, h2, h⟩
-  rw[Option.bind_eq_some_iff] at h; rcases h with ⟨_, h3, h⟩
-  rw[Option.bind_eq_some_iff] at h; rcases h with ⟨_, h4, h⟩
-  rw[Option.bind_eq_some_iff] at h; rcases h with ⟨_, h5, h⟩
-  rw[Option.bind_eq_some_iff] at h; rcases h with ⟨_, h6, h⟩
-  rw[Option.bind_eq_some_iff] at h; rcases h with ⟨_, h7, h⟩
-  rw[Option.bind_eq_some_iff] at h; rcases h with ⟨_, h8, h⟩
-  rw[Option.bind_eq_some_iff] at h; rcases h with ⟨_, h9, h⟩
-  cases h;
-  replace ih1 := ih1 h1; clear h1
-  replace ih2 := ih2 h5; clear h5
-  replace h2 := infer_kind_sound h2 wf
-  replace h3 := Ty.is_eq_some_sound h3
-  replace h4 := Kind.base_kind_sound h4
-  replace h6 := infer_kind_sound h6 wf
-  replace h7 := Ty.is_eq_some_sound h7
-  replace h8 := Kind.base_kind_sound h8
-  replace h9 := Kind.is_closed_kind_sound h9
-  subst h3; subst h7;
-  rw[h4] at ih1; rw[h4] at h2
-  rw[h9] at ih2; rw[h9] at h6
-  rw[h9] at h8; cases h8
-  apply Typing.arrowc
-  assumption
-  assumption
-
-case _ ih1 =>
-  rw[Option.bind_eq_some_iff] at h; rcases h with ⟨_, h1, h⟩
-  rw[Option.bind_eq_some_iff] at h; rcases h with ⟨_, h2, h⟩
-  rw[Option.bind_eq_some_iff] at h; rcases h with ⟨_, h3, h⟩
-  rw[Option.bind_eq_some_iff] at h; rcases h with ⟨_, h4, h⟩
-  rw[Option.bind_eq_some_iff] at h; rcases h with ⟨_, h5, h⟩
-  rw[Option.bind_eq_some_iff] at h; rcases h with ⟨_, h6, h⟩
-  rw[Option.bind_eq_some_iff] at h; rcases h with ⟨_, h7, h⟩
-  rw[Option.bind_eq_some_iff] at h; rcases h with ⟨_, h8, h⟩
-  rw[Option.bind_eq_some_iff] at h; rcases h with ⟨_, h9, h⟩
-  rw[Option.bind_eq_some_iff] at h; rcases h with ⟨_, h10, h⟩
-  simp at h; rcases h with ⟨h, e⟩; subst e
-  rcases h with ⟨h, e1⟩
-  rcases h with ⟨h, e2⟩
-  rcases h with ⟨h, e3⟩
-  rcases h with ⟨e4, e5⟩
-  subst e4; subst e3
-  replace ih1 := ih1 h1; clear h1
-  replace h2 := Ty.is_eq_some_sound h2
-  replace h3 := Ty.is_app_some_sound h3
-  replace h4 := Ty.is_app_some_sound h4
-  replace h5 := infer_kind_sound h5 wf
-  replace h6 := infer_kind_sound h6 wf
-  replace h7 := infer_kind_sound h7 wf
-  replace h8 := infer_kind_sound h8 wf
-  replace h9 := Kind.is_arrow_sound h9
-  replace h10 := Kind.is_arrow_sound h10
-  rw[e1] at e2;  rw[e1]
-  rw[e2]
-  rw[e5] at h7; rw[e5] at h8
-  subst h2; subst h9; subst h10
-  rw[h3] at ih1; rw [h4] at ih1
-  simp_all
-  apply Typing.fst
-  apply h7
-  apply h8
-  assumption
-
-case _ ih1 =>
-  rw[Option.bind_eq_some_iff] at h; rcases h with ⟨_, h1, h⟩
-  rw[Option.bind_eq_some_iff] at h; rcases h with ⟨_, h2, h⟩
-  rw[Option.bind_eq_some_iff] at h; rcases h with ⟨_, h3, h⟩
-  rw[Option.bind_eq_some_iff] at h; rcases h with ⟨_, h4, h⟩
-  rw[Option.bind_eq_some_iff] at h; rcases h with ⟨_, h5, h⟩
-  rw[Option.bind_eq_some_iff] at h; rcases h with ⟨_, h6, h⟩
-  rw[Option.bind_eq_some_iff] at h; rcases h with ⟨_, h7, h⟩
-  rw[Option.bind_eq_some_iff] at h; rcases h with ⟨_, h8, h⟩
-  rw[Option.bind_eq_some_iff] at h; rcases h with ⟨_, h9, h⟩
-  rw[Option.bind_eq_some_iff] at h; rcases h with ⟨_, h10, h⟩
-  simp at h; rcases h with ⟨h, e⟩; subst e
-  rcases h with ⟨h, e1⟩
-  rcases h with ⟨h, e2⟩
-  rcases h with ⟨h, e3⟩
-  rcases h with ⟨e4, e5⟩
-  subst e4; subst e3
-  replace ih1 := ih1 h1; clear h1
-  replace h2 := Ty.is_eq_some_sound h2
-  replace h3 := Ty.is_app_some_sound h3
-  replace h4 := Ty.is_app_some_sound h4
-  replace h5 := infer_kind_sound h5 wf
-  replace h6 := infer_kind_sound h6 wf
-  replace h7 := infer_kind_sound h7 wf
-  replace h8 := infer_kind_sound h8 wf
-  replace h9 := Kind.is_arrow_sound h9
-  replace h10 := Kind.is_arrow_sound h10
-  rw[e1] at e2;
-  rw[e5] at h7; rw[e5] at h8
-  subst h2; subst h9; subst h10
-  rw[h3] at ih1; rw [h4] at ih1
-  simp_all
-  apply Typing.snd
-  assumption
-  assumption
-  assumption
-case _ ih1 =>
-  rw[Option.bind_eq_some_iff] at h; rcases h with ⟨_, h1, h⟩
-  rw[Option.bind_eq_some_iff] at h; rcases h with ⟨_, h2, h⟩
-  rw[Option.bind_eq_some_iff] at h; rcases h with ⟨_, h3, h⟩
-  cases h
-  replace ih1 := ih1 h1; clear h1
-  replace h2 := Ty.is_eq_some_sound h2
-  replace h3 := Kind.is_closed_kind_sound h3
-  rw[h3] at h2; rw[h3]
-  subst h2
-  apply Typing.allc
-  assumption
-case _ ih1 ih2 =>
-  rw[Option.bind_eq_some_iff] at h; rcases h with ⟨_, h1, h⟩
-  rw[Option.bind_eq_some_iff] at h; rcases h with ⟨_, h2, h⟩
-  rw[Option.bind_eq_some_iff] at h; rcases h with ⟨_, h3, h⟩
-  rw[Option.bind_eq_some_iff] at h; rcases h with ⟨_, h4, h⟩
-  rw[Option.bind_eq_some_iff] at h; rcases h with ⟨_, h5, h⟩
-  rw[Option.bind_eq_some_iff] at h; rcases h with ⟨_, h6, h⟩
-  simp at h; rcases h with ⟨h, e⟩; subst e
-  rcases h with ⟨h, e1⟩; rcases h with ⟨e2, e3⟩
-  replace ih1 := ih1 h1; clear h1
-  replace h2 := Ty.is_eq_some_sound h2
-  replace h3 := Ty.is_all_some_sound h3
-  replace h4 := Ty.is_all_some_sound h4
-  replace h5 := ih2 h5
-  replace h6 := Ty.is_eq_some_sound h6
-  subst h2; subst h6
-  rw[e1] at ih1; rw[e2] at h3;  rw[e2] at e3
-  rw[h3] at ih1; rw[h4] at ih1
-  rw[e3] at h5
-  apply Typing.apptc
-  assumption
-  assumption
-  rfl
-  rfl
-case _ ih1 ih2 =>
-  rw[Option.bind_eq_some_iff] at h; rcases h with ⟨_, h1, h⟩
-  rw[Option.bind_eq_some_iff] at h; rcases h with ⟨_, h2, h⟩
-  rw[Option.bind_eq_some_iff] at h; rcases h with ⟨_, h3, h⟩
-  simp at h; cases h.1; cases h.2; clear h
-  replace ih1 := ih1 h1
-  replace ih2 := ih2 h2
-  replace h3 := infer_kind_sound h3 wf
-  apply Typing.choice
-  assumption
-  assumption
-  assumption
 end Core
